ETCSsettings.sml
@@ -1,3 +1,22 @@
+fun sspecl tl th = 
+    let val (b,vs) = strip_forall $ concl th
+        val ars = List.filter (fn (n,s) => not (on_ground o fst o dest_sort o snd $ (n,s))) vs
+        val env = match_tl essps (List.map mk_var ars) tl emptyvd
+        val tl' = List.map (inst_term env) (List.map mk_var vs)
+    in specl tl' th
+    end
+
+
+fun sspecl_then tl (ttac: thm_tactic): thm_tactic = 
+    fn th => ttac (sspecl tl th)
+
+val qsspecl_then = qterml_tcl sspecl_then
+
+
+
+
+
+
 fun store_as name th = 
 let val _ = store_thm(name, th)
 in th
