SEARList.sml
@@ -1,0 +1,112 @@
+
+val lemma = 
+ 
+
+
+(*
+
+[1,2]
+
+
+{(0,1),(1,2)}
+
+
+[2,1]
+
+
+{(0,2),(1,1)}
+
+
+N -> (A + 1)
+
+
+eq_psym
+
+
+a = c & b = d
+---------
+P(a,b) <=> P(c,d)
+
+
+
+
+fun eq_Pred p  = 
+
+
+
+?P
+
+
+
+
+()
+
+*)
+
+
+
+val lemma = 
+fVar_Inst 
+[("P",([("sets",mem_sort$ Pow $ Pow $ Cross N (mk_set "A"))],
+“IN(Empty(N * A),sets:mem(Pow(Pow(N * A)))) & 
+ !l. IN(l,sets) ==> !a:mem(A).IN(Ins(Pair(Card(l),a),l),sets)”))] 
+(IN_def_P_expand |> qspecl [‘Pow(Pow(N * A))’]) 
+
+(*make Ins Pair as Cons0 *)
+
+(*set of subsets of that contains the set of lists*)
+val As_def = lemma |> ex2fsym0 "As" ["A"] |> conjE1 
+                   |> gen_all |> GSYM
+
+
+
+val U_ex_lemma = fVar_Inst 
+[("P",([("ls",mem_sort $ Pow $ Cross N (mk_set "A"))],
+“IN(ls,BIGINTER(As(A)))”))]
+(Thm_2_4 |> qspecl [‘(Pow(N * A))’]) 
+|> conv_rule $ once_depth_fconv no_conv 
+$ rewr_fconv (spec_all IN_BIGINTER)
+|> conv_rule $ once_depth_fconv no_conv 
+$ rewr_fconv (spec_all As_def)
+
+
+
+
+(*f:A->B. is inj, then ?g:B->A. g o f = id(A).
+  
+have this function. 
+
+
+*)
+
+val U_i_def = U_ex_lemma |> ex2fsym0 "U" ["A"] |>ex2fsym0 "i" ["A"]
+
+
+
+val IN_U = U_i_def |> conjE2 |> gen_all |> 
+conv_rule $ basic_once_fconv no_conv (rewr_fconv (eq_sym "mem"))
+|> GSYM
+
+
+val List0 = IN_U  |> allE (rastt "A") |>  allE (rastt "Eval(i(A),b)")
+                       |> dimp_mp_l2r
+                       (existsI ("b'",mem_sort (rastt "U(A)")) 
+                                (rastt "b:mem(U(A))")
+                                “Eval(i(A), b') = Eval(i(A), b)”
+                                (refl (rastt "Eval(i(A), b)")))
+                       |> gen_all
+                       |> disch_all
+                       |> gen_all
+
+val List_lemma = prove_store("List_lemma",
+e0
+()
+(form_goal
+ “!A b. ”));
+
+
+val _ = new_pred "hasCard" [("xs",mem_sort $Pow (mk_set "X")),("n",mem_sort N)]
+val hasCard_def = store_ax("hasCard_def",
+“!X xs:mem(Pow(X)) n.hasCard(xs,n) <=> Holds(Card(X),xs,n)”)
+
+val Card_def' = Card_lemma |> rewr_rule[GSYM hasCard_def]
